src/Common/Literal.v
@@ -1,0 +1,14 @@
+From Utils Require Import Int.
+
+Inductive literal : Set := 
+| IntLit (n: int) 
+| BoolLit (b: bool)
+| UnitLit.
+
+Definition lit_eqb l1 l2 :=
+  match l1, l2 with
+  | IntLit n1, IntLit n2 => BinIntDef.Z.eqb n1 n2
+  | BoolLit b1, BoolLit b2 => Bool.eqb b1 b2
+  | UnitLit, UnitLit => true
+  | _, _ => false
+  end.
