src/Common/Primitive.v
@@ -1,0 +1,9 @@
+(* Unary and binary primitives are pure *)
+Inductive binary_primitives : Set := 
+| Add | Sub | Mul | Div | Mod 
+| Lt | Le | Eq
+| Or | And
+| Tup.
+
+Inductive unary_primitives : Set := 
+| Neg | Not | Fst | Snd | Left | Right | Id.
