src/utils/IO.v
@@ -1,0 +1,6 @@
+From Utils Require Import Int.
+
+Record IO := {input : list int; output : list int}.
+
+Definition outputs io o := 
+  {|input:= input io; output:= o::output io|}.
