src/utils/Tactics.v
@@ -2,8 +2,10 @@ Require Export Lia.
 
 #[global]
 Hint Extern 50 => lia: lia.
+#[global]
+Hint Extern 50 => exfalso: exfalso.
 
-Ltac destruct_exist :=
+Ltac destruct_exist_H :=
   match goal with 
   | H: exists _, _ |- _ => 
       destruct H
@@ -23,41 +25,84 @@ Ltac destruct_and_H :=
 
 Ltac invert H := inversion H; subst.
 
+Ltac rewrite_S n :=
+  let a := fresh "A" in
+  assert (a: S n = n + 1) by lia;
+  rewrite a in *; clear a.
+
 Ltac simpl_lia :=
   match goal with 
-  | H: ?n + 1 < ?m + 1 |- _ =>
+  | H: S ?n < S ?m |- _ =>
+      idtac "simpl 0";
+      let a := fresh "A" in
+      assert (a: n < m) by lia;
+      clear H
+  | H: ?n + 1 < S ?m |- _ =>
+      idtac "simpl 1";
+      let a := fresh "A" in
+      assert (a: n < m) by lia;
+      clear H
+  | H: ?n + ?k < ?m + ?k |- _ =>
+      idtac "simpl 2";
       let a := fresh "A" in
       assert (a: n < m) by lia;
       clear H
   | H: ?n + ?m < ?n + ?k |- _ =>
+      idtac "simpl 3";
       let a := fresh "A" in
       assert (a: m < k) by lia;
       clear H
   | H: ?n + ?m < ?n + ?k + ?l |- _ =>
+      idtac "simpl 4";
       let a := fresh "A" in
       assert (a: m < k + l) by lia;
       clear H
   | _ : context[?n + (?m + ?l)] |- _ => 
+      idtac "simpl 5";
       let e := fresh "E" in
       assert (e:n + (m + l) = n + m + l) by lia;
       rewrite e in *; clear e
   | |- context[?n + (?m + ?l)] => 
+      idtac "simpl 6";
       let e := fresh "E" in
       assert (e:n + (m + l) = n + m + l) by lia;
       rewrite e in *; clear e
   | H: ~ ?n < ?m |- _ =>
+      idtac "simpl 7";
       let e := fresh "E" in
       let n' := fresh n in
       assert (e: n = m + (n - m)) by lia;
       rewrite e in *; clear e H;
       set (n' := n - m) in *
-  | |- _ => lia
+  | H: context[?n + 0] |- _ => 
+      idtac "simpl 8";
+      let e := fresh "E" in
+      assert (e: n + 0 = n) by lia;
+      rewrite e in *; clear e
+  | [|- context[?n + 0]] => 
+      idtac "simpl 9";
+      let e := fresh "E" in
+      assert (e: n + 0 = n) by lia;
+      rewrite e in *; clear e
+  | H: context[0 + ?n] |- _ => 
+      idtac "simpl 10";
+      let e := fresh "E" in
+      assert (e: 0 + n = n) by lia;
+      rewrite e in *; clear e
+  | [|- context[0 + ?n]] => 
+      idtac "simpl 11";
+      let e := fresh "E" in
+      assert (e: 0 + n = n) by lia;
+      rewrite e in *; clear e
+  | |- _ => 
+      idtac "trying lia"; lia
   end.
 
 Ltac reduce :=
   intros || (cbn in *) || subst 
   || intuition congruence 
-  || destruct_exist || destruct_and_H.
+  || destruct_exist_H || destruct_and_H
+  || autounfold with *.
 
 Ltac destruct_match :=
   match goal with 
